platform/Depl/examples/Baby.v
@@ -1,6 +1,12 @@
 Require Import Depl.
 
 
+Module D.
+  Definition dom := Empty_set.
+End D.
+
+Module Import Depl := Depl.Make(D).
+
 (** * The simplest function possible *)
 
 Definition nada := dmodule "m" {{
@@ -80,7 +86,7 @@ Definition const := dmodule "m" {{
   dfunction "f" [
     ARGS()
     PRE Emp
-    POST |^fE, fE "result" = !(natToW 0)|
+    POST |^fE, fE "result" = $0|
   ]
     Return 0
   end
@@ -171,8 +177,8 @@ Qed.
 Definition starPure2 := dmodule "m" {{
   dfunction "f" [
     ARGS("x", "y", "z")
-    PRE (|^fE, fE "x0" = !(natToW 0)| * |^fE, fE "y0" = !(natToW 1)|) * |^fE, fE "z0" = !(natToW 2)|
-    POST |^fE, fE "z0" = !(natToW 2)| * (|^fE, fE "y0" = !(natToW 1)| * |^fE, fE "x0" = !(natToW 0)|)
+    PRE (|^fE, fE "x0" = $0| * |^fE, fE "y0" = $1|) * |^fE, fE "z0" = $2|
+    POST |^fE, fE "z0" = $2| * (|^fE, fE "y0" = $1| * |^fE, fE "x0" = $0|)
   ]
     Return 0
   end
